Weidenbach_Book/IsaSAT_Trail.thy
@@ -617,14 +617,14 @@ definition (in -) isa_length_trail_pre where
   \<open>isa_length_trail_pre = (\<lambda> (M', xs, lvls, reasons, k, cs). length M' \<le> uint32_max)\<close>
 
 definition (in -) isa_length_trail where
-  \<open>isa_length_trail = (\<lambda> (M', xs, lvls, reasons, k, cs). length_u M')\<close>
+  \<open>isa_length_trail = (\<lambda> (M', xs, lvls, reasons, k, cs). length_uint32_nat M')\<close>
 
 lemma isa_length_trail_pre:
   \<open>(M, M') \<in> trail_pol \<A> \<Longrightarrow> isa_length_trail_pre M\<close>
   by (auto simp: isa_length_trail_def trail_pol_alt_def isa_length_trail_pre_def)
 
 lemma isa_length_trail_length_u:
-  \<open>(RETURN o isa_length_trail, RETURN o length_u) \<in> trail_pol \<A> \<rightarrow>\<^sub>f \<langle>nat_rel\<rangle>nres_rel\<close>
+  \<open>(RETURN o isa_length_trail, RETURN o length_uint32_nat) \<in> trail_pol \<A> \<rightarrow>\<^sub>f \<langle>nat_rel\<rangle>nres_rel\<close>
   by (intro frefI nres_relI)
     (auto simp: isa_length_trail_def trail_pol_alt_def
     intro!: ASSERT_leI)
@@ -1565,7 +1565,7 @@ qed
 
 (* TODO: Kill the other definition *)
 lemma isa_length_trail_length_u_no_CS:
-  \<open>(RETURN o isa_length_trail, RETURN o length_u) \<in> trail_pol_no_CS \<A> \<rightarrow>\<^sub>f \<langle>nat_rel\<rangle>nres_rel\<close>
+  \<open>(RETURN o isa_length_trail, RETURN o length_uint32_nat) \<in> trail_pol_no_CS \<A> \<rightarrow>\<^sub>f \<langle>nat_rel\<rangle>nres_rel\<close>
   by (intro frefI nres_relI)
     (auto simp: isa_length_trail_def trail_pol_no_CS_alt_def ann_lits_split_reasons_def
       intro!: ASSERT_leI)
