Weidenbach_Book/IsaSAT_VMTF.thy
@@ -226,7 +226,7 @@ sepref_definition (in -) insert_sort_nth_code
       vmtf_conc\<^sup>k *\<^sub>a (arl_assn uint32_nat_assn)\<^sup>d  \<rightarrow>
        arl_assn uint32_nat_assn\<close>
   unfolding insert_sort_nth_def insert_sort_def insert_sort_inner_nth_def[symmetric]
-    length_u_def[symmetric] one_uint32_nat_def[symmetric]
+    length_uint32_nat_def[symmetric] one_uint32_nat_def[symmetric]
   supply [[goals_limit = 1]]
   supply mset_eq_setD[dest] mset_eq_length[dest]
   by sepref
@@ -603,7 +603,7 @@ sepref_definition isa_vmtf_flush_code
   supply vmtf_en_dequeue_pre_def[simp] vmtf_insert_sort_nth_code_preD[dest] le_uint32_max_le_uint64_max[intro]
   unfolding vmtf_flush_def PR_CONST_def isa_vmtf_flush_int_def zero_uint32_nat_def[symmetric]
     current_stamp_def[symmetric] one_uint32_nat_def[symmetric]
-  apply (rewrite at \<open>\<lambda>(i, vm, h). _ < \<hole>\<close> length_u_def[symmetric])
+  apply (rewrite at \<open>\<lambda>(i, vm, h). _ < \<hole>\<close> length_uint32_nat_def[symmetric])
   apply (rewrite at \<open>length _ + \<hole>\<close> nat_of_uint64_conv_def[symmetric])
   by sepref
 
@@ -617,7 +617,7 @@ sepref_definition isa_vmtf_flush_fast_code
   supply vmtf_en_dequeue_pre_def[simp] vmtf_insert_sort_nth_code_preD[dest] le_uint32_max_le_uint64_max[intro]
   unfolding isa_vmtf_flush_int_def PR_CONST_def vmtf_flush_int_def zero_uint32_nat_def[symmetric]
     current_stamp_def[symmetric] one_uint32_nat_def[symmetric]
-  apply (rewrite at \<open>\<lambda>(i, vm, h). _ < \<hole>\<close> length_u_def[symmetric])
+  apply (rewrite at \<open>\<lambda>(i, vm, h). _ < \<hole>\<close> length_uint32_nat_def[symmetric])
   apply (rewrite at \<open>length _ + \<hole>\<close> nat_of_uint64_conv_def[symmetric])
   by sepref
 
